Making Reg concrete x86_64 register variants
- Making Reg an enum of concrete register variants in the x86_64
  architecture.
- Added a function to do initialization of the Register Allocator state.

crates/cachet-compiler/src/bpl.rs
@@ -2267,6 +2267,7 @@ lazy_static! {
             (Ident::from("initInputOperandLocation").into(), Proc),
             (Ident::from("initValueInputOperandLocation").into(), Proc),
             (Ident::from("initValueReg").into(), Proc),
+            (Ident::from("initRegState").into(), Proc),
         ])
     };
 
